allow names for nonrep and same shape

case_studies/POPLmark/Pattern.thy
@@ -1,6 +1,14 @@
 theory Pattern
-  imports POPLmark_1B "HOL-ex.Sketch_and_Explore"
+  imports POPLmark_1B
+  keywords "linearize_mrbnf" :: thy_goal
 begin
+
+
+definition asSS :: "('a \<Rightarrow> 'a) \<Rightarrow> 'a \<Rightarrow> 'a" where
+  "asSS f \<equiv> if |supp f| <o |UNIV :: 'a set| then f else id"
+
+ML_file "../../Tools/mrbnf_linearize_tactics.ML"
+ML_file "../../Tools/mrbnf_linearize.ML"
 
 setup \<open>Sign.qualified_path false (Binding.name "P")\<close>
 
@@ -126,23 +134,23 @@ declare [[ML_print_depth=1000]]
 linearize_mrbnf (PTVars: 'tv::var, PVars: 'v::var) pat = "('tv::var, 'v::var) prepat"
   [wits:"(PPRec lfempty) :: ('tv::var, 'v::var) prepat"] on 'v
   for map: vvsubst_pat
-subgoal for R x y
+  subgoal for R x y
     apply (unfold P.Pattern.P.prepat.in_rel mem_Collect_eq map_vvsubst_equiv)
     apply (rule iffI)
-      apply (auto)
+     apply (auto)
     subgoal for b P Q
       apply (hypsubst_thin)
       apply (drule trans)
-      apply (rule sym)
-      apply (assumption)
+       apply (rule sym)
+       apply (assumption)
       apply (drule trans)
-      apply (rule sym)
+       apply (rule sym)
        apply (assumption)
       apply (erule thin_rl)
       apply (rotate_tac 2)
       apply (erule thin_rl)
       apply (erule thin_rl)
-      proof (induction P arbitrary: Q)
+    proof (induction P arbitrary: Q)
       case (PPVar x T)
       then show ?case
         apply (cases Q)
@@ -154,10 +162,9 @@ subgoal for R x y
         apply (cases Q)
          apply (auto)
         apply (unfold map_vvsubst_equiv[symmetric] id_def[symmetric])
-        thm lfset.inj_map_strong
         subgoal for X'
-        apply (rule lfset_inj_map_strong2[of X X' "(map_prepat fst)" "(map_prepat fst)"
-              "(map_prepat snd)" "(map_prepat snd)"])
+          apply (rule lfset_inj_map_strong2[of X X' "(map_prepat fst)" "(map_prepat fst)"
+                "(map_prepat snd)" "(map_prepat snd)"])
             apply (auto)
           apply (blast)
           done
@@ -165,17 +172,16 @@ subgoal for R x y
     qed
     done
   subgoal
-    apply (rule ex_nonrep_prepat[unfolded map_vvsubst_equiv])
+    apply (unfold prepat.in_rel[OF supp_id_bound, unfolded prepat.map_id])
+    apply (intro allI impI exI[of _ id])
+    apply (unfold prepat.map_id)
+    apply (auto)
+    apply (rule trans[OF sym, rotated])
+     apply assumption
+    apply (rule prepat.map_cong; (rule supp_id_bound refl)?)
+    apply (drule arg_cong[where f=PPVars])
+    apply (simp add: prepat.set_map)
     done
-  apply (unfold prepat.in_rel[OF supp_id_bound, unfolded prepat.map_id])
-  apply (intro allI impI exI[of _ id])
-  apply (unfold prepat.map_id)
-  apply (auto)
-  apply (rule trans[OF sym, rotated])
-   apply assumption
-  apply (rule prepat.map_cong; (rule supp_id_bound refl)?)
-  apply (drule arg_cong[where f=PPVars])
-  apply (simp add: prepat.set_map)
   done
 
 lemma nonrep_prepat_def_alt: "nonrep_prepat (x :: ('tv::var, 'v::var) prepat) 
