operations/Linearize_alist.thy
@@ -1,0 +1,1004 @@
+theory Linearize_alist
+  imports "Binders.MRBNF_Composition" "Binders.MRBNF_Recursor"
+begin
+
+definition asSS :: "('a \<Rightarrow> 'a) \<Rightarrow> 'a \<Rightarrow> 'a" where
+  "asSS f \<equiv> if |supp f| <o |UNIV :: 'a set| then f else id"
+
+declare [[mrbnf_internals]]
+declare [[ML_print_depth=10000]]
+
+
+(* LIST *)
+lemma "\<And> R (x :: 'a list) y. list_all2 R x y = (\<exists>z. set z \<subseteq> {(x, y). R x y} \<and> map fst z = x \<and> map snd z = y)"
+  subgoal for R x y
+    apply (rule list.in_rel[of R x y, unfolded mem_Collect_eq])
+    done
+  done
+
+definition sameShape_list :: "'a list \<Rightarrow> 'a list \<Rightarrow> bool" where 
+  "sameShape_list x x' \<equiv> list_all2 top x x'"
+
+definition nonrep_list :: "'a list \<Rightarrow> bool" where 
+  "nonrep_list x \<equiv> \<forall> x'. sameShape_list x x' \<longrightarrow> (\<exists> f. x' = map f x)"
+
+lemma sameShape_list_alt: "list_all2 top xs xs' = (length xs = length xs')"
+  by (simp add: list_all2_conv_all_nth)
+
+lemma ex_not: "((\<forall>x. P x) \<longrightarrow> False) = (\<exists>x. \<not>P x)"
+  by simp
+
+lemma "nonrep_list [1::nat, 1, 1] \<longrightarrow> False"
+  apply (unfold nonrep_list_def sameShape_list_def sameShape_list_alt)
+  apply (rule ex_not[THEN iffD2])
+  apply (rule exI[of _ "[1, 2, 3]"])
+  apply (auto)
+  done
+
+lemma "nonrep_list [1::nat, 2, 3]"
+  apply (unfold nonrep_list_def sameShape_list_def sameShape_list_alt)
+  apply (rule allI)
+  apply (rule impI)
+  subgoal for x
+    apply (rule exI[of _ "(\<lambda> y. (if y = 1 then (hd x) else (if y = 2 then (hd (tl x)) else (hd (tl (tl x))))))"])
+    apply (auto)
+    by (metis (lifting) ext length_0_conv length_Suc_conv list.sel(1,3))
+  done
+
+(* PROD *)
+print_bnfs
+
+definition sameShape_prod_1 :: "('a \<times> 'b) \<Rightarrow> ('a \<times> 'b) \<Rightarrow> bool" where 
+  "sameShape_prod_1 x x' \<equiv> rel_prod top (=) x x'"
+
+definition nonrep_prod_1 :: "('a \<times> 'b) \<Rightarrow> bool" where 
+  "nonrep_prod_1 x \<equiv> \<forall> x'. sameShape_prod_1 x x' \<longrightarrow> (\<exists> f. x' = map_prod f id x)"
+
+lemma "nonrep_prod_1 (a, b)"
+  apply (unfold nonrep_prod_1_def sameShape_prod_1_def)
+  apply (auto)
+  done
+
+typedef 'a nrp_list = "{(xs :: 'a list). nonrep_list xs}"
+  apply (rule exI[of _ "[]"])
+  apply (auto simp add: nonrep_list_def sameShape_list_def)
+  done
+
+
+mrbnf "'a list"
+  map: map
+    sets: set
+  bd: "natLeq"
+  oops
+
+bnf "'a list"
+  map: map
+    sets: set
+  bd: "natLeq"
+          apply(auto simp add: infinite_regular_card_order_natLeq[unfolded infinite_regular_card_order_def]  list.set_bd)
+  sorry
+print_theorems
+
+local_setup \<open>
+fn ctxt => 
+  let
+    val ((mrbnf,_), (_,ctxt)) = MRBNF_Comp.mrbnf_of_typ true MRBNF_Def.Smart_Inline
+      (I) flat [] [] [] @{typ "('k \<times> 'v) list"}
+      ((MRBNF_Comp.empty_comp_cache, MRBNF_Comp.empty_unfolds), ctxt) |> @{print};
+  in                                                 
+    MRBNF_Def.register_mrbnf Plugin_Name.default_filter "pre_alist" mrbnf ctxt
+  end
+\<close>
+
+print_mrbnfs
+
+
+(*linearize_mrbnf ('k::var,'v) alist = "('k::var \<times> 'v) list" on 'k*)
+
+(*
+mrbnf pre_alist: "('k \<times> 'v) list"
+  map: map_pre_alist
+    sets: live: keys live: vals
+  bd: "natLeq"
+         apply (auto simp add: map_prod_compose map_pre_alist_def)
+         apply (unfold keys_def vals_def)[]
+  apply (simp)
+  apply (metis fst_conv image_eqI)
+         apply (unfold keys_def vals_def)[]
+  apply (simp)
+        apply (metis snd_conv image_eqI)
+  subgoal sorry
+  subgoal sorry
+     apply (simp add: infinite_regular_card_order_natLeq)
+  sorry
+print_theorems*)
+ 
+definition keys :: "('k \<times> 'v) list \<Rightarrow> 'k set" where
+  "keys l \<equiv> set (map fst l)"
+
+definition vals :: "('k \<times> 'v) list \<Rightarrow> 'v set" where
+  "vals l \<equiv> set (map snd l)"
+
+definition map_pre_alist :: "('k \<Rightarrow> 'k') \<Rightarrow> ('v \<Rightarrow> 'v') \<Rightarrow> ('k \<times> 'v) list \<Rightarrow> ('k' \<times> 'v') list" where
+  "map_pre_alist f g l \<equiv> map (map_prod f g) l"
+
+
+definition rrel_pre_alist :: "('k \<Rightarrow> 'k' \<Rightarrow> bool) \<Rightarrow> ('v \<Rightarrow> 'v' \<Rightarrow> bool) 
+  \<Rightarrow> ('k \<times> 'v) list \<Rightarrow> ('k' \<times> 'v') list \<Rightarrow> bool" where
+  "rrel_pre_alist R S l l' \<equiv> mr_rel_list (\<lambda> x x'. R (fst x) (fst x') \<and>  S (snd x) (snd x')) l l'"
+
+axiomatization where
+  (* The next property assumes preservation of pullbacks on the third position. 
+   NB: All MRBNFs already preserve _weak_ pullbacks, i.e., they satisfy the following property 
+   without uniqueness.  *)
+  F_rel_map_set2_strong: 
+  "\<And> R S (x :: (('k \<times> 'v) list)) y.
+    rrel_pre_alist R S x y =
+      (\<exists>!z. keys z \<subseteq> {(x, y). R x y} \<and>
+            vals z \<subseteq> {(x, y). S x y} \<and> map_pre_alist fst fst z = x \<and> map_pre_alist snd snd z = y)"
+  and
+  (* The next property assumes that nonrepetitive elements exist: *)
+  ex_nonrep: "\<exists>x. \<forall>x'. rrel_pre_alist top (=) x x' \<longrightarrow> (\<exists> f. x' = map_pre_alist f id x)"
+
+(* Important consequence of preservation of pullbacks (which is actually equivalent to it): 
+The relator is closed under intersections. *)
+
+lemma pre_alist_strong:
+  "rrel_pre_alist R3 R4 x y \<Longrightarrow> rrel_pre_alist Q3 Q4 x y \<Longrightarrow> rrel_pre_alist (inf R3 Q3) (inf R4 Q4) x y"
+  thm list.mr_rel_mono_strong0
+  apply (unfold rrel_pre_alist_def)
+  apply (frule list.mr_rel_mono_strong0)
+   apply (intro ballI impI)
+  apply (rule trans[OF top_apply[THEN fun_cong] trans[OF top_apply top_bool_def]])
+  apply(rotate_tac 2)
+  apply (unfold F.map_id mr_rel_F_def eq_True)
+  thm F_rel_map_set2_strong
+  apply (drule F_rel_map_set2_strong[THEN iffD1])
+  apply (unfold top_apply top_bool_def Collect_const_case_prod if_True eqTrueI[OF subset_UNIV] simp_thms(22))
+  apply (unfold F.in_rel[OF supp_id_bound bij_id supp_id_bound, unfolded id_apply F.map_id OO_Grp_alt]
+      id_def[symmetric] mem_Collect_eq)
+  apply (elim exE alt_ex1E)
+  apply (erule conjE)
+  apply (erule conjE)
+  apply (erule conjE)
+  apply (erule conjE)
+  apply (erule conjE)
+  apply (erule conjE)
+  apply (erule conjE)
+  subgoal premises subprems for z l r
+    thm subprems
+    apply (insert spec2[OF subprems(1), of r z]
+        spec2[OF subprems(1), of l z]; (erule impE); (erule impE))
+       apply (rule conjI; rule conjI; rule subprems)
+       apply (rule conjI; rule conjI; rule subprems)
+       apply (rule conjI; rule conjI; rule subprems)
+    apply (rule exI)
+    apply (unfold inf_fun_def inf_bool_def)
+    apply (rule conjI)
+     apply (insert subprems) []
+     apply (hypsubst_thin)
+    apply ((rule conjI)?,
+        rule subrelI, 
+        rule CollectI, 
+        rule case_prodI, 
+        (rule conjI; erule rev_subsetD[THEN iffD1[OF prod_in_Collect_iff]]),
+        assumption, assumption)+
+    apply (rule conjI)
+    apply (rule subprems)+
+    done
+  done
+
+ML \<open>
+open BNF_Util BNF_Tactics
+
+fun mk_rel_F_exchange_tac mrbnf F_mr_rel_mono_strong0 F_strong ctxt =
+  let
+    val id_prems = MRBNF_Comp_Tactics.mk_id_prems mrbnf;
+  in
+    HEADGOAL (Subgoal.FOCUS
+      (fn {prems, context = ctxt, ...} => 
+        HEADGOAL (EVERY' [
+          rtac ctxt (F_mr_rel_mono_strong0 OF flat (replicate 2 id_prems)),
+          rtac ctxt (F_strong OF prems),
+          K (unfold_thms_tac ctxt ([id_apply, eqTrueI OF [refl]] @ @{thms ball_triv inf_apply inf_bool_def}))
+        ]) THEN
+        ALLGOALS (
+          (rtac ctxt impI THEN' 
+          rtac ctxt TrueI) ORELSE'
+          (rtac ctxt ballI THEN' 
+          rtac ctxt ballI THEN'
+          rtac ctxt impI THEN'
+          eresolve_tac ctxt [conjunct1, conjunct2]))
+       ) ctxt)
+  end
+\<close>
+
+(* lin_pos dependent? *)
+(* Another important consequence: the following "exchange"-property, which could be read: 
+Since the atoms have a fixed position, we can permute the relations: *)
+lemma rel_F_exchange: 
+  fixes x :: "('a1::var,'a2::var,'a3,'a4) F" and x' :: "('a1,'a2,'a3','a4') F"
+  assumes "rel_F id id R3 R4 x x'" and "rel_F id id Q3 Q4 x x'"
+  shows "rel_F id id R3 Q4 x x'" 
+  using assms apply -
+  apply (tactic \<open>mk_rel_F_exchange_tac (MRBNF_Def.mrbnf_of @{context} @{type_name F} |> the) 
+    @{thm F.mr_rel_mono_strong0} @{thm F_strong} @{context} 
+    THEN print_tac @{context} "done" THEN no_tac\<close>)
+  subgoal premises prems
+    apply (rule F.mr_rel_mono_strong0[OF supp_id_bound bij_id supp_id_bound supp_id_bound bij_id supp_id_bound])
+    apply (rule F_strong[OF prems])
+       apply (unfold id_apply eqTrueI[OF refl] ball_triv inf_apply inf_bool_def)
+       apply (intro impI TrueI)+
+     apply (intro ballI impI; erule conjunct1 conjunct2)+
+    done
+  done
+
+(* Then notion of two items having the same shape (w.r.t. the 3rd position): *)
+(* these definitions are lin_pos dependent *)
+definition sameShape1 :: "('a1::var,'a2::var,'a3,'a4) F \<Rightarrow> ('a1,'a2,'a3,'a4) F \<Rightarrow> bool" where 
+  "sameShape1 x x' \<equiv> rel_F id id top (=) x x'"
+
+definition nonrep2 :: "('a1::var,'a2::var,'a3,'a4) F \<Rightarrow> bool" where 
+  "nonrep2 x \<equiv> \<forall> x'. sameShape1 x x' \<longrightarrow> (\<exists> f. x' = map_F id id f id x)"
+
+ML\<open>
+open BNF_Util BNF_Tactics
+
+fun mk_nonrep2_map_F_tac mrbnf nonrep_def sameShape_def F_map_comp F_mr_rel_map mr_rel_F_def F_rel_compp 
+  F_rel_Grp F_map_id F_in_rel F_rel_maps F_rel_refl_strong ctxt = 
+  HEADGOAL (Subgoal.FOCUS 
+    (fn {prems, context = ctxt, ...} => 
+      let
+        val var_types = var_types_of_mrbnf mrbnf;
+        val nr_lives = length (filter (fn v => v = MRBNF_Def.Live_Var) var_types);
+        val nr_non_lives = length (filter (fn v => not (v = MRBNF_Def.Live_Var)) var_types);
+        val lin_live_pos = fold_index (fn (i, v) => fn b => 
+          if (v = MRBNF_Def.Live_Var andalso i+1 < lin_pos) then b+1 else b) var_types 1;
+        val switch_poses = map_range (fn i => if i < (lin_pos-(lin_live_pos)) then i+1 else i+2) (nr_non_lives);
+        val switch = (fn thm1 => (fn thm2 => trans OF [thm1, thm2 RS sym]));
+        val o_id = @{thm o_id};
+        val id_o = @{thm id_o};
+      in
+        unfold_thms_tac ctxt [nonrep_def, sameShape_def] THEN
+        HEADGOAL (EVERY' [
+          rtac ctxt allI,
+          rtac ctxt impI,
+          etac ctxt exE,
+          EqSubst.eqsubst_tac ctxt [0] [F_map_comp] THEN_ALL_NEW
+            TRY o resolve_tac ctxt (prems @ @{thms supp_id_bound bij_id}),
+          K (unfold_thms_tac ctxt [switch id_o o_id]),
+          EqSubst.eqsubst_tac ctxt [lin_pos] [switch o_id id_o], (*move all id to the right except for lin_pos*)
+          EqSubst.eqsubst_tac ctxt [0] [F_map_comp RS sym] THEN_ALL_NEW
+            TRY o resolve_tac ctxt (prems @ @{thms supp_id_bound bij_id}),
+          dtac ctxt (rotate_prems ~1 (F_mr_rel_map RS iffD1)) THEN_ALL_NEW
+            TRY o resolve_tac ctxt (prems @ @{thms supp_id_bound bij_id}),
+          K (unfold_thms_tac ctxt [switch id_o o_id, @{thm Grp_UNIV_id}]),
+          K (unfold_thms_tac ctxt [switch @{thm OO_eq} @{thm eq_OO}]),  
+          EqSubst.eqsubst_asm_tac ctxt [lin_live_pos] [switch @{thm eq_OO} @{thm OO_eq}], (*move all (=) to the left except for lin_live_pos*)
+          K (unfold_thms_tac ctxt @{thms eq_alt}),   
+          EqSubst.eqsubst_tac ctxt [0] @{thms Grp_UNIV_id}
+        ]) THEN
+        unfold_thms_tac ctxt [mr_rel_F_def, o_id, F_rel_compp, F_rel_Grp] THEN
+        unfold_thms_tac ctxt [eqTrueI OF @{thms subset_UNIV}, @{thm simp_thms(21)}, id_o, @{thm UNIV_def} RS sym] THEN
+        unfold_thms_tac ctxt ([eqTrueI OF [@{thm UNIV_I}], id_apply] @ @{thms Grp_UNIV_id OO_def Grp_def simp_thms(21)}) THEN
+        HEADGOAL (EVERY' [
+          etac ctxt exE,
+          etac ctxt conjE,
+          dtac ctxt (rotate_prems ~1 (F_in_rel RS iffD1)) THEN_ALL_NEW
+            TRY o resolve_tac ctxt prems,
+          Method.insert_tac ctxt [unfold_thms ctxt [nonrep_def, sameShape_def, mr_rel_F_def, F_map_id] 
+            (nth prems (length prems -1))],
+          etac ctxt exE,
+          etac ctxt conjE,
+          etac ctxt CollectE,
+          etac ctxt conjE
+        ]) THEN
+        REPEAT_DETERM_N (nr_lives-1) (HEADGOAL (
+          etac ctxt conjE)) THEN
+        HEADGOAL (hyp_subst_tac_thin true ctxt) THEN
+        HEADGOAL (Subgoal.FOCUS 
+          (fn {prems = subprems, context = ctxt, params, ...} => 
+            HEADGOAL (EVERY' [
+              Method.insert_tac ctxt [nth subprems 0],
+              etac ctxt allE,
+              etac ctxt impE,
+              rtac ctxt (infer_instantiate' ctxt [NONE, SOME (snd (nth params 1))] exI),
+              EqSubst.eqsubst_tac ctxt [1] [nth F_rel_maps 0],
+              EqSubst.eqsubst_tac ctxt [1] [nth F_rel_maps 1]
+            ]) THEN
+            HEADGOAL (rtac ctxt F_rel_refl_strong) THEN
+            REPEAT_DETERM_N nr_lives (HEADGOAL (
+                (dresolve_tac ctxt (map (fn p => subsetD OF [p] RS @{thm Collect_case_prodD}) (drop 1 subprems)) THEN'
+                  (assume_tac ctxt ORELSE' 
+                  (rtac ctxt sym THEN' assume_tac ctxt))))) THEN
+            HEADGOAL (EVERY' [
+              etac ctxt exE,
+              EqSubst.eqsubst_tac ctxt [0] [F_map_comp] THEN_ALL_NEW
+                TRY o resolve_tac ctxt (prems @ @{thms supp_id_bound bij_id}),
+              EqSubst.eqsubst_tac ctxt switch_poses [switch id_o o_id],
+              EqSubst.eqsubst_tac ctxt [0] [F_map_comp RS sym] THEN_ALL_NEW
+                TRY o resolve_tac ctxt (prems @ @{thms supp_id_bound bij_id}),
+              rtac ctxt exI,
+              dtac ctxt arg_cong,
+              assume_tac ctxt
+            ]) 
+          ) ctxt)
+      end)
+  ctxt)
+\<close>
+
+lemma nonrep2_map_F:
+  fixes x :: "('a1::var,'a2::var,'a3,'a4) F"
+    and v :: "'a1 \<Rightarrow> 'a1" and u :: "'a2\<Rightarrow>'a2" and g :: "'a4 \<Rightarrow> 'b4"
+  assumes v: "|supp v| <o |UNIV :: 'a1 set|"  and u: "bij u" "|supp u| <o |UNIV :: 'a2 set|" 
+  assumes "nonrep2 x"
+  shows "nonrep2 (map_F v u id g x)"
+  using assms apply -
+  subgoal premises prems
+    apply (unfold nonrep2_def sameShape1_def)
+    apply (rule allI)
+    apply (rule impI)
+    apply (subst F.map_comp; (rule prems bij_id supp_id_bound)?)
+    apply (unfold o_id id_o)
+    apply (drule iffD1[OF F.mr_rel_map(1), rotated -1]; (rule prems bij_id supp_id_bound)?)
+    apply (unfold trans[OF id_o o_id[symmetric]] Grp_UNIV_id trans[OF OO_eq eq_OO[symmetric]])
+    apply (unfold trans[OF eq_OO OO_eq[symmetric], of top])
+    apply (unfold eq_alt)
+    apply (subst Grp_UNIV_id)
+    apply (unfold mr_rel_F_def o_id F.rel_compp F.rel_Grp)
+    apply (unfold eqTrueI[OF subset_UNIV] simp_thms(21) UNIV_def[symmetric] id_o)
+    apply (unfold Grp_UNIV_id OO_def Grp_def eqTrueI[OF UNIV_I] simp_thms(21) id_apply)
+    apply (unfold id_def[THEN sym])
+    apply (erule exE)
+    apply (erule conjE)
+    apply (drule F.in_rel[THEN iffD1, rotated -1]; (rule prems)?)
+    apply (erule exE)
+    apply (erule conjE)
+    apply (erule CollectE)
+    apply (erule conjE)
+    apply (erule conjE)
+    apply (insert prems(4)[unfolded nonrep2_def sameShape1_def mr_rel_F_def F.map_id])
+    apply (rotate_tac -1)
+    apply (hypsubst_thin)
+    subgoal premises subprems for x' y z
+      apply (insert subprems(1))
+      apply (erule allE)
+      apply (erule impE)
+       apply (subst F.rel_map)
+       apply (subst F.rel_map)
+       apply (rule F.rel_refl_strong)
+        apply (drule subsetD[OF subprems(2), THEN Collect_case_prodD] 
+          subsetD[OF subprems(3), THEN Collect_case_prodD]; 
+          (assumption)?; (rule sym; assumption)?)+
+      apply (elim exE)
+      apply (subst F.map_comp[OF _ _ _ supp_id_bound bij_id supp_id_bound, unfolded trans[OF id_o o_id[symmetric]]]; (rule prems)?)
+      apply (subst F.map_comp[THEN sym]; (rule prems bij_id supp_id_bound)?)
+      subgoal premises subprems for f
+        apply (rule exI[of _ f]) (* instantiation not necessary but easy*)
+        apply (subst subprems)
+        apply (subst F.map_comp; (rule prems bij_id supp_id_bound)?)
+        apply (unfold o_id id_o)
+        apply (rule refl)
+        done
+      done
+    done
+  done
+
+ML\<open>
+open BNF_Util BNF_Tactics
+
+fun mk_nonrep2_map_F_rev_tac mrbnf nonrep_def sameShape_def F_mr_rel_map1 F_mr_rel_map2 F_mr_rel_map3 F_map_comp F_rel_eq 
+  F_mr_rel_id rel_F_exchange F_mr_rel_flip F_mr_rel_mono_strong0 F_mr_rel_Grp ctxt = 
+  HEADGOAL (Subgoal.FOCUS 
+    (fn {prems, context = ctxt, ...} => 
+      let
+        val var_types = var_types_of_mrbnf mrbnf;
+        val nr_lives = length (filter (fn v => v = MRBNF_Def.Live_Var) var_types);
+        val nr_non_lives = length (filter (fn v => not (v = MRBNF_Def.Live_Var)) var_types);
+        val lin_live_pos = fold_index (fn (i, v) => fn b => 
+          if (v = MRBNF_Def.Live_Var andalso i+1 < lin_pos) then b+1 else b) var_types 1;
+        val switch = (fn thm1 => (fn thm2 => trans OF [thm1, thm2 RS sym]));
+      in
+        unfold_thms_tac ctxt [nonrep_def, sameShape_def] THEN
+        HEADGOAL (EVERY' [
+          rtac ctxt allI,
+          rtac ctxt impI,
+          etac ctxt exE,
+          forward_tac ctxt [rotate_prems ~1 F_mr_rel_map2] THEN_ALL_NEW
+            TRY o resolve_tac ctxt (prems @ @{thms supp_id_bound bij_id}),
+          rotate_tac 1,
+          EqSubst.eqsubst_asm_tac ctxt (map_range (fn i => i+1) nr_non_lives) [switch @{thm o_id} @{thm id_o}],
+          EqSubst.eqsubst_asm_tac ctxt [lin_live_pos] @{thms Grp_UNIV_id},
+          K (unfold_thms_tac ctxt [switch @{thm eq_OO} @{thm OO_eq}]),
+          EqSubst.eqsubst_asm_tac ctxt [lin_live_pos] [switch @{thm OO_eq} @{thm eq_OO}], (*move all (=) to the right and then lin_live_pos back*)
+          EqSubst.eqsubst_asm_tac ctxt [lin_live_pos] @{thms eq_alt},
+          EqSubst.eqsubst_asm_tac ctxt [0] [F_mr_rel_map1 RS sym] THEN_ALL_NEW
+            TRY o resolve_tac ctxt (prems @ @{thms supp_id_bound bij_id}),
+          Method.insert_tac ctxt [unfold_thms ctxt [nonrep_def, sameShape_def] (nth prems (length prems - 1))],
+          etac ctxt allE,
+          etac ctxt impE,
+          rtac ctxt exI,
+          assume_tac ctxt,
+          etac ctxt thin_rl,
+          etac ctxt exE,
+          EqSubst.eqsubst_asm_tac ctxt [0] [F_map_comp] THEN_ALL_NEW
+            TRY o resolve_tac ctxt (prems @ @{thms supp_id_bound bij_id}),
+          K (unfold_thms_tac ctxt @{thms id_o o_id}),
+          EqSubst.eqsubst_asm_tac ctxt [1] [F_rel_eq RS sym],
+          EqSubst.eqsubst_asm_tac ctxt [1] [F_mr_rel_id],
+          dtac ctxt (rotate_prems ~1 (iffD1 OF [F_mr_rel_map1])) THEN_ALL_NEW
+            TRY o resolve_tac ctxt (prems @ @{thms supp_id_bound bij_id}),
+          K (unfold_thms_tac ctxt @{thms id_o OO_eq}),
+          dtac ctxt (rotate_prems 1 rel_F_exchange),
+          rtac ctxt (F_mr_rel_flip RS iffD1) THEN_ALL_NEW
+            TRY o resolve_tac ctxt @{thms supp_id_bound bij_id},
+          K (unfold_thms_tac ctxt @{thms inv_id}),
+          EqSubst.eqsubst_asm_tac ctxt [0] [F_mr_rel_map3] THEN_ALL_NEW
+            TRY o resolve_tac ctxt (prems @ @{thms supp_id_bound bij_id}),
+          EqSubst.eqsubst_asm_tac ctxt (map_range (fn i => i+1) (2 * nr_lives)) @{thms Grp_def},
+          EqSubst.eqsubst_asm_tac ctxt (map_range (fn i => i+1) (nr_non_lives)) @{thms inv_o_simp1} THEN_ALL_NEW
+            TRY o resolve_tac ctxt (@{thm bij_id}::prems),
+          K (unfold_thms_tac ctxt ((eqTrueI OF @{thms UNIV_I}):: @{thms id_apply simp_thms(21)})),
+          EqSubst.eqsubst_asm_tac ctxt [lin_live_pos] @{thms eq_commute},
+          K (unfold_thms_tac ctxt @{thms eq_OO conversep_def}),
+          etac ctxt (rotate_prems (~1 - (length var_types)) F_mr_rel_mono_strong0) THEN_ALL_NEW
+            TRY o resolve_tac ctxt @{thms supp_id_bound bij_id}
+        ]) THEN
+        REPEAT_DETERM_N (length var_types) (
+          (HEADGOAL (
+            (* for bound and free *)
+            rtac ctxt ballI THEN'
+            rtac ctxt refl)) 
+          ORELSE 
+          (HEADGOAL (
+            (* for lives*)
+            rtac ctxt ballI THEN'
+            rtac ctxt ballI THEN'
+            rtac ctxt impI THEN'
+            rotate_tac 2 THEN'
+            EqSubst.eqsubst_asm_tac ctxt [0] @{thms eq_commute} THEN'
+            assume_tac ctxt))
+        ) THEN
+        HEADGOAL (EVERY' [
+          etac ctxt thin_rl,
+          EqSubst.eqsubst_asm_tac ctxt [lin_live_pos] [@{thm Grp_UNIV_def} RS sym],
+          rtac ctxt exI,
+          EqSubst.eqsubst_asm_tac ctxt (map_range (fn i => i+1) (nr_lives -1)) @{thms eq_alt},
+          EqSubst.eqsubst_asm_tac ctxt [0] [F_mr_rel_Grp] THEN_ALL_NEW
+            TRY o resolve_tac ctxt @{thms supp_id_bound bij_id}
+        ]) THEN
+        unfold_thms_tac ctxt ([eqTrueI OF @{thms subset_UNIV}, eqTrueI OF @{thms UNIV_I}, @{thm UNIV_def} RS sym] @ 
+          @{thms simp_thms(21) Grp_def}) THEN
+        HEADGOAL (assume_tac ctxt)
+      end)
+  ctxt)
+\<close>
+
+(* Here we need pullback preservation: *)
+lemma nonrep2_map_F_rev:
+  fixes x :: "('a1::var,'a2::var,'a3,'a4) F" and u :: "'a2\<Rightarrow>'a2" and g :: "'a4 \<Rightarrow> 'a4'"
+  assumes u: "bij u" "|supp u| <o |UNIV :: 'a2 set|" 
+  assumes "nonrep2 (map_F id u id g x)"
+  shows "nonrep2 x"
+  using assms apply -
+ (* apply (tactic \<open>mk_nonrep2_map_F_rev_tac (MRBNF_Def.mrbnf_of @{context} @{type_name F} |> the) @{thm nonrep2_def} @{thm sameShape1_def} @{thm F.mr_rel_map(1)}
+    @{thm F.mr_rel_map(2)} @{thm F.mr_rel_map(3)} @{thm F.map_comp} @{thm F.rel_eq} @{thm F.mr_rel_id} @{thm rel_F_exchange} 
+    @{thm F.mr_rel_flip} @{thm F.mr_rel_mono_strong0} @{thm F.mr_rel_Grp} @{context} 
+    THEN print_tac @{context} "done" THEN no_tac\<close>)*)
+  subgoal premises prems
+    apply (unfold nonrep2_def sameShape1_def)
+    apply (rule allI)
+    apply (rule impI)
+
+(* alt *)
+    apply (insert prems(3)[unfolded nonrep2_def sameShape1_def]) (*lastprem*)
+    apply (elim allE impE)
+     apply (rule F.mr_rel_map(1)[THEN iffD2]; (rule prems supp_id_bound bij_id)?)
+  (*_ * (2*nr_BF + nr_As + 2(x,y)) *)
+   apply (drule F.mr_rel_map(2)[rotated -1, of _ _ _ _ _ _ _ _ id _]; (rule prems supp_id_bound bij_id)?)
+     apply (unfold o_id id_o Grp_UNIV_id eq_OO OO_eq)
+     apply (assumption)
+
+    apply (erule exE)
+    apply (subst (asm) F.map_comp; (rule prems supp_id_bound bij_id)?)
+    apply (unfold o_id id_o)
+
+    thm F.map_cong
+
+    apply (subst (asm) F.rel_eq[symmetric])
+    apply (unfold F.mr_rel_id)
+    thm F.mr_rel_map
+    apply (drule iffD1[OF F.mr_rel_map(1), rotated -1]; (rule prems supp_id_bound bij_id)?)
+    apply (unfold id_o OO_eq)
+    thm rel_F_exchange[rotated]
+    apply (drule rel_F_exchange[rotated])
+     apply (rule iffD1[OF F.mr_rel_flip]; (rule supp_id_bound bij_id)?)
+    apply (unfold inv_id)
+     apply (subst (asm) F.mr_rel_map(3); (rule prems supp_id_bound bij_id)?)
+     apply (unfold Grp_def)
+    apply (subst (asm) (1 2) inv_o_simp1; (rule prems bij_id)?) (*for all frees and bounds*)
+     apply (tactic \<open>unfold_thms_tac @{context} @{thms eqTrueI[OF UNIV_I] simp_thms(21) id_apply}\<close>) (*for all frees*)
+     apply (subst (asm) eq_commute) (*lin_live_pos*)
+     apply (unfold eq_OO conversep_def)
+     apply (elim F.mr_rel_mono_strong0[rotated -5]; (rule supp_id_bound bij_id)?) (*- len vartypes - 1*)
+      (*left subtactic is for frees and bounds, right subtactic for lives*)
+    apply ((rule ballI,rule refl)?; (rule ballI,rule ballI,rule impI,rotate_tac 2,subst (asm) eq_commute,assumption))+
+
+    apply (erule thin_rl)
+    apply (subst (asm) Grp_UNIV_def[symmetric]) (*lin_live_pos*)
+    apply (rule exI)
+    apply (subst (asm) eq_alt) (* repeat lives - 1 *)
+    thm F.mr_rel_Grp
+    apply (subst (asm) F.mr_rel_Grp; (rule supp_id_bound bij_id)?)
+    apply (unfold eqTrueI[OF subset_UNIV] eqTrueI[OF UNIV_I] UNIV_def[THEN sym] simp_thms(21) Grp_def)
+    apply (assumption)
+    done
+  done
+
+ML\<open>
+open BNF_Util BNF_Tactics
+fun mk_nonrep2_map_bij_tac nonrep_def sameShape_def F_mr_rel_map1 F_map_comp cgs ctxt = 
+  HEADGOAL (Subgoal.FOCUS 
+    (fn {prems, context = ctxt, ...} => 
+      unfold_thms_tac ctxt [nonrep_def, sameShape_def] THEN
+      HEADGOAL (EVERY' [
+        rtac ctxt allI,
+        rtac ctxt impI,
+        dtac ctxt (rotate_prems ~1 (F_mr_rel_map1 RS iffD1)) THEN_ALL_NEW
+          TRY o resolve_tac ctxt @{thms bij_id supp_id_bound},
+        K (unfold_thms_tac ctxt @{thms o_id Grp_UNIV_id eq_OO Grp_OO_top}),
+        dtac ctxt (Object_Logic.rulify ctxt (unfold_thms ctxt [nonrep_def, sameShape_def] (nth prems 1))),
+        etac ctxt exE,
+        hyp_subst_tac_thin true ctxt
+      ]) THEN
+      unfold_thms_tac ctxt @{thms triv_forall_equality} THEN
+      HEADGOAL (Subgoal.FOCUS 
+        (fn {context = ctxt, params, ...} => 
+          HEADGOAL (EVERY' (map (fn ((_, cf), cg) => 
+            let
+              val g = Thm.term_of cg
+              val (dom_g, rng_g) = fastype_of g |> dest_funT
+              val inv_g = Const ("Hilbert_Choice.inv", 
+                (fastype_of g) --> (rng_g --> dom_g)) $ g
+              val f_o_inv_g = HOLogic.mk_comp (Thm.term_of cf, inv_g)
+            in
+              rtac ctxt (infer_instantiate' ctxt [NONE, SOME (Thm.cterm_of ctxt f_o_inv_g)] exI) 
+            end) (params ~~ cgs))
+          ) THEN
+          HEADGOAL (rtac ctxt sym) THEN
+          HEADGOAL (rtac ctxt trans) THEN
+          HEADGOAL (rtac ctxt F_map_comp THEN_ALL_NEW
+            TRY o resolve_tac ctxt @{thms bij_id supp_id_bound}) THEN
+          unfold_thms_tac ctxt ([@{thm inv_o_simp1} OF (take 1 prems), @{thm o_assoc} RS sym] @ @{thms id_o o_id}) THEN
+          HEADGOAL (rtac ctxt refl)
+        ) ctxt)
+  ) ctxt)
+\<close>
+
+lemma nonrep2_mapF_bij:
+  fixes x :: "('a1::var,'a2::var,'a3,'a4) F" and g::"'a3\<Rightarrow>'a3"
+  assumes g: "bij g" and x: "nonrep2 x"
+  shows "nonrep2 (map_F id id g id x)" (is "nonrep2 ?x'")
+  using assms apply -
+  apply (tactic \<open>mk_nonrep2_map_bij_tac @{thm nonrep2_def}
+    @{thm sameShape1_def} @{thm F.mr_rel_map(1)} @{thm F.map_comp} [@{cterm g}] @{context}
+    THEN print_tac @{context} "done" THEN no_tac\<close>) 
+  subgoal premises prems
+    apply (unfold nonrep2_def sameShape1_def)
+    apply (rule allI)
+    apply (rule impI)
+    apply (drule F.mr_rel_map(1)[THEN iffD1, rotated -1]; (rule supp_id_bound bij_id)?)
+    apply (unfold o_id Grp_UNIV_id eq_OO Grp_OO_top)
+    apply (drule x[unfolded nonrep2_def sameShape1_def, rule_format])
+    apply (erule exE conjE)+
+    apply hypsubst_thin
+    subgoal for _ f
+      apply (rule exI[of _ "f o inv g"])
+      apply (rule sym)
+      apply (rule trans)
+       apply (rule F.map_comp; (rule supp_id_bound bij_id)?)
+      apply (unfold id_o o_id inv_o_simp1[OF g] o_assoc[symmetric])
+      apply (rule refl)
+      done
+    done
+  done
+
+ML \<open>
+open BNF_Util BNF_Tactics
+
+fun mk_nonrep2_mapF_bij_2_tac mrbnf nonrep2_mapF_bij nonrep2_map_F F_map_comp ctxt =
+  HEADGOAL (Subgoal.FOCUS
+    (fn {prems, context = ctxt, ...} => 
+    let val nr_prems = length prems;
+        val id_prems = MRBNF_Comp_Tactics.mk_id_prems mrbnf;
+    in
+      HEADGOAL (rtac ctxt (unfold_thms ctxt ((F_map_comp OF ((take (nr_prems-2) prems) @ id_prems)) :: @{thms id_o o_id}) 
+        (nonrep2_mapF_bij OF [nth prems (nr_prems-2), nonrep2_map_F OF (nth_drop (nr_prems-2) prems)])
+      ))
+     end) ctxt)
+\<close>
+
+lemma nonrep2_mapF_bij_2:
+  fixes x :: "('a1::var,'a2::var,'a3,'a4) F"
+    and v :: "'a1 \<Rightarrow> 'a1" and u :: "'a2\<Rightarrow>'a2" and g::"'a3\<Rightarrow>'a3" and f::"'a4\<Rightarrow>'a4'"
+  assumes v: "|supp v| <o |UNIV :: 'a1 set|" and u: "bij u" "|supp u| <o |UNIV :: 'a2 set|"
+    and g: "bij g" and x: "nonrep2 x"
+  shows "nonrep2 (map_F v u g f x)" 
+  using assms apply -
+  apply (tactic \<open>mk_nonrep2_mapF_bij_2_tac (MRBNF_Def.mrbnf_of @{context} @{type_name F} |> the) 
+    @{thm nonrep2_mapF_bij} @{thm nonrep2_map_F} @{thm F.map_comp} @{context} 
+    THEN print_tac @{context} "done" THEN no_tac\<close>)
+  subgoal premises prems
+    apply (rule nonrep2_mapF_bij[OF prems(4) nonrep2_map_F[OF prems(1,2,3,5)], 
+          unfolded F.map_comp[OF prems(1,2,3) supp_id_bound bij_id supp_id_bound] id_o o_id])
+    done
+  done
+
+
+typedef ('a1::var,'a2::var,'a3::var,'a4) F' = "{x :: ('a1,'a2,'a3,'a4) F. nonrep2 x}"
+  apply (unfold mem_Collect_eq nonrep2_def sameShape1_def mr_rel_F_def F.map_id)
+  by (rule ex_nonrep)
+
+definition set1_F' :: "('a1::var,'a2::var,'a3::var,'a4) F' \<Rightarrow> 'a1 set" where "set1_F' = set1_F o Rep_F'"
+definition set2_F' :: "('a1::var,'a2::var,'a3::var,'a4) F' \<Rightarrow> 'a2 set" where "set2_F' = set2_F o Rep_F'"
+definition set3_F' :: "('a1::var,'a2::var,'a3::var,'a4) F' \<Rightarrow> 'a3 set" where "set3_F' = set3_F o Rep_F'"
+definition set4_F' :: "('a1::var,'a2::var,'a3::var,'a4) F' \<Rightarrow> 'a4 set" where "set4_F' = set4_F o Rep_F'"
+
+definition map_F' :: "('a1::var \<Rightarrow> 'a1) \<Rightarrow> ('a2::var \<Rightarrow> 'a2) \<Rightarrow> ('a3::var \<Rightarrow> 'a3) \<Rightarrow> ('a4 \<Rightarrow> 'a4') 
+  \<Rightarrow> ('a1,'a2,'a3,'a4) F' \<Rightarrow> ('a1,'a2,'a3,'a4') F'"
+  where "map_F' v u f g = Abs_F' o map_F (asSS v) (asSS (asBij u)) (asBij f) g o Rep_F'"
+
+definition rrel_F' :: "('a4 \<Rightarrow> 'a4' \<Rightarrow> bool) \<Rightarrow> ('a1::var,'a2::var,'a3::var,'a4) F' \<Rightarrow> ('a1,'a2,'a3,'a4') F' \<Rightarrow> bool"
+  where "rrel_F' R x x' = rrel_F (=) R (Rep_F' x) (Rep_F' x')"
+
+(* Verifying the axioms of a MRBNF for F':  *)
+lemma F'_map_id: "map_F' id id id id = id"
+  apply (unfold map_F'_def asSS_def asBij_def 
+      eqTrueI[OF bij_id] eqTrueI[OF supp_id_bound] if_True)
+  apply (rule ext)
+  apply (unfold o_apply F.map_id Rep_F'_inverse)
+  apply (unfold id_def)
+  apply (rule refl)
+  done
+
+lemma F'_map_comp1_:
+  fixes u1 v1 :: "'a1::var \<Rightarrow> 'a1"
+  fixes u2 v2 :: "'a2::var \<Rightarrow> 'a2"
+  fixes u3 v3 :: "'a3::var \<Rightarrow> 'a3"
+  assumes "|supp u1| <o |UNIV :: 'a1 set|" "|supp v1| <o |UNIV :: 'a1 set|"
+  assumes "bij u2" "|supp u2| <o |UNIV :: 'a2 set|" "bij v2" "|supp v2| <o |UNIV :: 'a2 set|"
+  assumes "bij u3" "|supp u3| <o |UNIV :: 'a3 set|" "bij v3" "|supp v3| <o |UNIV :: 'a3 set|"
+  shows "map_F' (v1 o u1) (v2 o u2) (v3 o u3) (g o f) = map_F' v1 v2 v3 g o map_F' u1 u2 u3 f"
+  using assms apply -
+  subgoal premises prems
+    apply (unfold map_F'_def asBij_def asSS_def)
+    apply (unfold eqTrueI[OF bij_comp[OF prems (3, 5)]] eqTrueI[OF bij_comp[OF prems (7, 9)]] 
+        eqTrueI[OF supp_comp_bound[OF prems(1,2) infinite_UNIV]] eqTrueI[OF supp_comp_bound[OF prems(4,6) infinite_UNIV]]
+        if_True)
+    apply (unfold 
+        eqTrueI[OF assms(1)] eqTrueI[OF assms(2)] eqTrueI[OF assms(3)] eqTrueI[OF assms(4)] eqTrueI[OF assms(5)] eqTrueI[OF assms(6)]
+        eqTrueI[OF assms(7)] eqTrueI[OF assms(8)] eqTrueI[OF assms(9)] eqTrueI[OF assms(10)]
+        if_True)
+    apply (rule ext)
+    apply (subst F.map_comp0; (rule prems)?)
+    apply (unfold o_apply)
+    apply (subst Abs_F'_inverse[unfolded mem_Collect_eq])
+     apply (rule nonrep2_mapF_bij_2; (rule prems Rep_F'[unfolded mem_Collect_eq])?)
+    apply (rule refl)
+    done
+  done
+
+
+(* This tactic is applicable to all 4 of the following <F'_setx_map_> lemmas*)
+ML \<open>
+open BNF_Util BNF_Tactics
+
+fun mk_set_map_tac set_F'_def map_F'_def Abs_F'_inverse Rep_F' nonrep2_mapF_bij_2 F_set_map ctxt =
+  HEADGOAL (Subgoal.FOCUS
+    (fn {prems = prems, context = ctxt, ...} =>
+      unfold_thms_tac ctxt ([set_F'_def, map_F'_def] @ map (fn thm => thm RS eqTrueI) prems @
+        @{thms asSS_def asBij_def if_True o_apply}) THEN
+      HEADGOAL (EVERY' [EqSubst.eqsubst_tac ctxt [0] [Abs_F'_inverse],
+        rtac ctxt nonrep2_mapF_bij_2 THEN_ALL_NEW resolve_tac ctxt (Rep_F' :: prems),
+        rtac ctxt F_set_map THEN_ALL_NEW
+          resolve_tac ctxt prems])
+    ) ctxt)
+\<close>
+
+lemma F'_set1_map_:
+  fixes u1 :: "'a1::var \<Rightarrow> 'a1"
+  fixes u2 :: "'a2::var \<Rightarrow> 'a2"
+  fixes u3 :: "'a3::var \<Rightarrow> 'a3"
+  assumes "|supp u1| <o |UNIV :: 'a1 set|"
+  assumes "bij u2" "|supp u2| <o |UNIV :: 'a2 set|"
+  assumes "bij u3" "|supp u3| <o |UNIV :: 'a3 set|"
+  shows "set1_F' (map_F' u1 u2 u3 f b) = u1 ` set1_F' b"
+  using assms apply -
+  apply (tactic \<open>mk_set_map_tac @{thm set1_F'_def} @{thm map_F'_def} @{thm Abs_F'_inverse[unfolded mem_Collect_eq]}
+    @{thm Rep_F'[unfolded mem_Collect_eq]} @{thm nonrep2_mapF_bij_2} @{thm F.set_map(1)} @{context} 
+    THEN print_tac @{context} "done" THEN no_tac\<close>)
+  subgoal premises prems
+    apply (unfold set1_F'_def map_F'_def asSS_def asBij_def
+        eqTrueI[OF prems(1)] eqTrueI[OF prems(2)] eqTrueI[OF prems(3)] eqTrueI[OF prems(4)] eqTrueI[OF prems(5)] o_apply if_True)
+    apply (subst Abs_F'_inverse[unfolded mem_Collect_eq])
+     apply (rule nonrep2_mapF_bij_2; (rule prems Rep_F'[unfolded mem_Collect_eq])?)
+    apply (rule F.set_map(1); (rule prems))
+    done
+  done
+
+lemma F'_set2_map_:
+  fixes u1 :: "'a1::var \<Rightarrow> 'a1"
+  fixes u2 :: "'a2::var \<Rightarrow> 'a2"
+  fixes u3 :: "'a3::var \<Rightarrow> 'a3"
+  assumes "|supp u1| <o |UNIV :: 'a1 set|"
+  assumes "bij u2" "|supp u2| <o |UNIV :: 'a2 set|"
+  assumes "bij u3" "|supp u3| <o |UNIV :: 'a3 set|"
+  shows "set2_F' (map_F' u1 u2 u3 f b) = u2 ` set2_F' b"
+  using assms apply -
+  apply (tactic \<open>mk_set_map_tac @{thm set2_F'_def} @{thm map_F'_def} @{thm Abs_F'_inverse[unfolded mem_Collect_eq]}
+    @{thm Rep_F'[unfolded mem_Collect_eq]} @{thm nonrep2_mapF_bij_2} @{thm F.set_map(2)} @{context}\<close>)
+  done
+
+lemma F'_set3_map_:
+  fixes u1 :: "'a1::var \<Rightarrow> 'a1"
+  fixes u2 :: "'a2::var \<Rightarrow> 'a2"
+  fixes u3 :: "'a3::var \<Rightarrow> 'a3"
+  assumes "|supp u1| <o |UNIV :: 'a1 set|"
+  assumes "bij u2" "|supp u2| <o |UNIV :: 'a2 set|"
+  assumes "bij u3" "|supp u3| <o |UNIV :: 'a3 set|"
+  shows "set3_F' (map_F' u1 u2 u3 f b) = u3 ` set3_F' b"
+  using assms apply -
+  apply (tactic \<open>mk_set_map_tac @{thm set3_F'_def} @{thm map_F'_def} @{thm Abs_F'_inverse[unfolded mem_Collect_eq]}
+    @{thm Rep_F'[unfolded mem_Collect_eq]} @{thm nonrep2_mapF_bij_2} @{thm F.set_map(3)} @{context}\<close>)
+  done
+
+lemma F'_set4_map_:
+  fixes u1 :: "'a1::var \<Rightarrow> 'a1"
+  fixes u2 :: "'a2::var \<Rightarrow> 'a2"
+  fixes u3 :: "'a3::var \<Rightarrow> 'a3"
+  assumes "|supp u1| <o |UNIV :: 'a1 set|"
+  assumes "bij u2" "|supp u2| <o |UNIV :: 'a2 set|"
+  assumes "bij u3" "|supp u3| <o |UNIV :: 'a3 set|"
+  shows "set4_F' (map_F' u1 u2 u3 f b) = f ` set4_F' b"
+  using assms apply -
+  apply (tactic \<open>mk_set_map_tac @{thm set4_F'_def} @{thm map_F'_def} @{thm Abs_F'_inverse[unfolded mem_Collect_eq]}
+    @{thm Rep_F'[unfolded mem_Collect_eq]} @{thm nonrep2_mapF_bij_2} @{thm F.set_map(4)} @{context}\<close>)
+  done
+
+lemma F'_map_cong_[fundef_cong]:
+  fixes u1 v1 :: "'a1::var \<Rightarrow> 'a1"
+  fixes u2 v2 :: "'a2::var \<Rightarrow> 'a2"
+  fixes u3 v3 :: "'a3::var \<Rightarrow> 'a3"
+  assumes "|supp u1| <o |UNIV :: 'a1 set|" "|supp v1| <o |UNIV :: 'a1 set|"
+  assumes "bij u2" "|supp u2| <o |UNIV :: 'a2 set|" "bij v2" "|supp v2| <o |UNIV :: 'a2 set|"
+  assumes "bij u3" "|supp u3| <o |UNIV :: 'a3 set|" "bij v3" "|supp v3| <o |UNIV :: 'a3 set|"
+    and "\<forall> a \<in> set1_F' x. u1 a = v1 a"
+    and "\<forall> a \<in> set2_F' x. u2 a = v2 a"
+    and "\<forall> a \<in> set3_F' x. u3 a = v3 a"
+    and "\<forall> a \<in> set4_F' x. f a = g a"
+  shows "map_F' u1 u2 u3 f x = map_F' v1 v2 v3 g x"
+  using assms apply -
+  subgoal premises prems
+    apply (unfold map_F'_def asSS_def asBij_def 
+        eqTrueI[OF assms(1)] eqTrueI[OF assms(2)] eqTrueI[OF assms(3)] eqTrueI[OF assms(4)] eqTrueI[OF assms(5)] 
+        eqTrueI[OF assms(6)] eqTrueI[OF assms(7)] eqTrueI[OF assms(8)] eqTrueI[OF assms(9)] eqTrueI[OF assms(10)]
+        eqTrueI[OF assms(11)] eqTrueI[OF assms(12)] eqTrueI[OF assms(13)] eqTrueI[OF assms(14)] if_True o_apply)
+    apply (subst F.map_cong; (rule prems(14,13,12,11,10,9,8,7,6,5,4,3,2,1))?) (*reverse prems so that the v-prems apply before the u-prems*)
+         apply (rule refl)
+         apply (erule bspec[OF prems(11)[unfolded set1_F'_def o_apply]] 
+        bspec[OF prems(12)[unfolded set2_F'_def o_apply]]
+        bspec[OF prems(13)[unfolded set3_F'_def o_apply]]
+        bspec[OF prems(14)[unfolded set4_F'_def o_apply]])+
+    apply (rule refl)
+    done
+  done
+
+lemma F'_set1_bd: "\<And>b. |set1_F' b| <o natLeq"
+  apply (unfold set1_F'_def o_apply)
+  by (rule F.set_bd(1))
+
+lemma F'_set2_bd: "\<And>b. |set2_F' b| <o natLeq"
+  apply (unfold set2_F'_def o_apply)
+  by (rule F.set_bd(2))
+
+lemma F'_set3_bd: "\<And>b. |set3_F' b| <o natLeq"
+  apply (unfold set3_F'_def o_apply)
+  by (rule F.set_bd(3))
+
+lemma F'_set4_bd: "\<And>b. |set4_F' b| <o natLeq"
+  apply (unfold set4_F'_def o_apply)
+  by (rule F.set_bd(4))
+
+lemma F'_rel_comp_leq_: "rrel_F' Q OO rrel_F' R \<le> rrel_F' (Q OO R)"
+  apply (rule predicate2I)
+  apply (erule relcomppE)
+  apply (unfold rrel_F'_def)
+  subgoal premises prems for x y b
+    apply (insert prems(1))
+    apply (drule relcomppI[of _ "Rep_F' x" "Rep_F' b" _ "Rep_F' y"])
+     apply (rule prems(2))
+    apply (unfold F.rel_compp[symmetric] eq_OO)
+    apply (assumption)
+    done
+  done
+
+lemma rrel_F_map_F3:
+  fixes x :: "('a :: var,'b :: var,'c,'d) F"
+  shows "rrel_F (Grp (f :: 'c \<Rightarrow> 'c)) R x y = rrel_F (=) R (map_F id id f id x) y"
+  apply (unfold F.rel_map(1) Grp_def id_apply eqTrueI[OF UNIV_I] simp_thms(21))
+  apply (rule iffI)
+   apply (erule F.rel_mono_strong; (assumption?, (erule sym)?))+
+  done
+
+lemma F'_in_rel:
+  fixes u1 :: "'a1::var \<Rightarrow> 'a1"
+  fixes u2 :: "'a2::var \<Rightarrow> 'a2"
+  fixes u3 :: "'a3::var \<Rightarrow> 'a3"
+  assumes u1: "|supp u1| <o |UNIV :: 'a1 set|"
+    and u2: "bij u2" "|supp u2| <o |UNIV :: 'a2 set|" 
+    and u3: "bij u3" "|supp u3| <o |UNIV :: 'a3 set|"
+  shows "rrel_F' R (map_F' u1 u2 u3 id x) y =
+    (\<exists>z. set4_F' z \<subseteq> {(x, y). R x y} \<and> map_F' id id id fst z = x \<and> map_F' u1 u2 u3 snd z = y)"
+  using assms apply -
+  subgoal premises prems
+    apply (unfold rrel_F'_def set4_F'_def map_F'_def asSS_def asBij_def if_True 
+        eqTrueI[OF prems(1)] eqTrueI[OF prems(2)] eqTrueI[OF prems(3)] eqTrueI[OF prems(4)] 
+        eqTrueI[OF prems(5)]
+        eqTrueI[OF supp_id_bound] eqTrueI[OF bij_id] o_apply)
+    apply (subst Abs_F'_inverse[unfolded mem_Collect_eq])
+     apply (rule nonrep2_mapF_bij_2; (rule prems Rep_F'[unfolded mem_Collect_eq])?)
+
+(* instantiation for bounds B, frees F, lives A: [_ * nr_BFs @ id * nr_BFs @ _ * nr_As @ id * nr_As] *)
+    apply (subst F.map_comp[of _ _ id id _ _ id id, unfolded o_id id_o, symmetric]; (rule prems bij_id supp_id_bound)?)
+    apply (subst rrel_F_map_F3[symmetric])
+    apply (subst F.in_rel; (rule prems)?)
+
+    apply (rule iffI)
+    apply (unfold Grp_def eqTrueI[OF UNIV_I] simp_thms(21))
+     apply (erule exE)
+     apply (erule conjE)
+     apply (erule conjE)
+     apply (erule CollectE)
+     apply (erule conjE)
+    subgoal premises subprems for z
+   apply (rule exI[of _ "(Abs_F' (map_F id id fst id z))"])
+      apply ((subst Abs_F'_inverse[unfolded mem_Collect_eq]), (tactic \<open>defer_tac 1\<close>))+ 
+         apply (tactic \<open>distinct_subgoals_tac\<close>)
+      prefer 2
+       apply (rule nonrep2_map_F_rev; (rule bij_id supp_id_bound)?)
+       apply (subst F.map_comp; (rule bij_id supp_id_bound)?)
+       apply (unfold o_id id_o)
+       apply (subst subprems)
+      apply (rule Rep_F'[unfolded mem_Collect_eq])
+
+      apply (subst (1 2) F.map_comp; (rule supp_id_bound bij_id prems)?)
+      apply (unfold o_id id_o)
+      apply (rule conjI)
+      apply ((rule conjI)?,
+        (subst F.set_map; (rule supp_id_bound bij_id)?),
+        subst image_id,
+        rule subprems)+
+      apply (rule conjI)
+       apply (subst subprems)
+       apply (rule Rep_F'_inverse[unfolded mem_Collect_eq])
+
+      apply (subst (2) Rep_F'_inverse[symmetric])
+      apply (subst subprems(2)[symmetric])
+      apply (rule F.map_cong[THEN arg_cong]; (rule prems refl)?)
+      apply (drule rev_subsetD[THEN Collect_case_prodD])
+       apply (rule subprems)
+      apply (rule sym)
+      apply (subst o_apply)
+      apply (assumption)
+      done
+    apply (erule exE)
+    apply (erule conjE)
+    apply (erule conjE)
+    apply (hypsubst_thin)
+    subgoal premises subprems for z
+      apply (rule exI)
+      apply (subst Abs_F'_inverse[unfolded mem_Collect_eq])
+       apply (rule nonrep2_mapF_bij_2; (rule supp_id_bound bij_id Rep_F'[unfolded mem_Collect_eq])?)
+      apply (rule conjI; (rule conjI)?)
+
+        prefer 3(* subgoal 3 is solvable without the exI instantiation and it "instantiates" ?z 
+          so that the other 2 subgoals are solvable as well*)
+        apply (subst Abs_F'_inverse[unfolded mem_Collect_eq])
+         apply (rule nonrep2_mapF_bij_2; (rule prems Rep_F'[unfolded mem_Collect_eq])?)
+        apply (subst F.map_comp; (rule bij_id supp_id_bound prems)?) (*having the id prems before the actual prems is important!*)
+        apply (unfold o_id)
+        apply (unfold o_def)
+        apply (rule F.map_cong; (rule prems refl)?)
+        apply (rule snd_conv)
+
+       apply (rule CollectI)
+       apply (subst F.set_map; (rule bij_id supp_id_bound)?)+
+       apply (unfold image_ident)
+       apply (rule conjI; (rule subprems)?)+
+        apply (rule subsetI)
+        apply (erule imageE)
+        apply (rule CollectI)
+       apply (rule case_prodI2)
+        apply (drule trans[OF sym, THEN iffD1[OF prod.inject]])
+         apply (assumption)
+        apply (erule conjE)
+        apply (rule trans[OF sym])
+         apply (assumption)
+        apply (erule arg_cong)
+
+      apply (subst F.map_comp; (rule supp_id_bound bij_id)?)
+      apply (unfold o_def fst_conv id_def)
+      apply (rule refl)
+      done
+    done
+  done
+
+ML \<open>
+open BNF_Util BNF_Tactics
+
+fun mk_strong_tac rrel_F'_def mr_rel_F_def F_strong F_map_id ctxt =
+  HEADGOAL (Subgoal.FOCUS
+    (fn {prems, context = ctxt, ...} => 
+    let
+      val _ = prems |> map @{print tracing}
+    in
+      unfold_thms_tac ctxt [rrel_F'_def] THEN
+      HEADGOAL (rtac ctxt (unfold_thms ctxt @{thms inf.idem} 
+        (unfold_thms ctxt [mr_rel_F_def, F_map_id] F_strong
+         OF (map (fn prem => unfold_thms ctxt [rrel_F'_def] prem) prems))))
+    end) ctxt)
+\<close>
+
+lemma F'_strong:
+  assumes "rrel_F' R x x'" 
+    and "rrel_F' Q x x'"
+  shows "rrel_F' (inf R Q) x x'" 
+  using assms apply -
+  apply (tactic \<open>mk_strong_tac @{thm rrel_F'_def} @{thm mr_rel_F_def} @{thm F_strong} @{thm F.map_id} @{context} 
+    THEN print_tac @{context} "done" THEN no_tac\<close>)
+  subgoal premises prems
+    apply (unfold rrel_F'_def)
+    apply (rule F_strong[unfolded mr_rel_F_def F.map_id, 
+          OF prems(1)[unfolded rrel_F'_def] prems(2)[unfolded rrel_F'_def], 
+          unfolded inf.idem])
+    done
+  done
+
+mrbnf "('a::var, 'b::var, 'c::var, 'd) F'"
+  map: map_F'
+  sets: free: set1_F' bound: set2_F' bound: set3_F' live: set4_F'
+  bd: natLeq
+  rel: rrel_F'
+  var_class: var
+
+  subgoal by (rule F'_map_id)
+  subgoal premises prems by (rule F'_map_comp1_; (rule prems))
+  subgoal premises prems 
+    apply (rule F'_map_cong_; (rule prems ballI)?)
+    by (rule prems, assumption)+
+  subgoal premises prems 
+    apply (rule ext)
+    apply (unfold o_apply)
+    by(rule F'_set1_map_[OF prems])
+  subgoal premises prems
+    apply (rule ext)
+    apply (unfold o_apply F'_set2_map_[OF prems]) 
+    by(rule refl)
+  subgoal premises prems 
+    apply (rule ext)
+    apply (unfold o_apply F'_set3_map_[OF prems]) 
+    by(rule refl)
+  subgoal premises prems 
+    apply (rule ext)
+    apply (unfold o_apply F'_set4_map_[OF prems]) 
+    by(rule refl)
+  subgoal by (rule infinite_regular_card_order_natLeq)
+  subgoal by (rule F'_set1_bd)
+  subgoal by (rule F'_set2_bd)
+  subgoal by (rule F'_set3_bd)
+  subgoal by (rule F'_set4_bd)
+  subgoal by (rule F'_rel_comp_leq_)
+  subgoal premises prems by (rule F'_in_rel[OF prems])
+  done        
+
+end
